\documentclass[class=jsarticle, crop=false, dvipdfmx, fleqn]{standalone}
\input{/Users/User/Documents/TeX/preamble/mypreamble}
\begin{document}
\section*{練習問題2-4}
\subsection*{1.}
\begin{comment}
\begin{equation}
V(a \cdot X + b) = a^2 \cdot V(X)
\end{equation}
を示す。
\end{comment}

$X$の平均を$\mu_X\ (= E[X])$，$u = a \cdot X + b$とおく。
$u$の平均は，期待値の性質を用いて，
\begin{equation}
\begin{split}
\mu_u & = E[u] = E[a \cdot X + b] \\
	& = a \cdot E[X] + b \\
	& = a \mu_X + b
\end{split}
\end{equation}
よって，$V(X) = E[(X - \mu_X)^2]$であることに注意して，
\begin{equation}
\begin{split}
V(a \cdot X + b) & = V(u) = E[(u - \mu_u)^2] \\
	& = E[\qty{(aX + b) - (a \mu_X+ b)}^2] \\
	& = E[(aX - a \mu_X)^2] \\
	& = E[a^2 (X - \mu_X)^2] \\
	& = a^2 E[(X - \mu_X)^2] \\
	& = a^2 V(X)
\end{split}
\end{equation}


\subsection*{2.}
$Z = X + Y$とおく。
$Z$の平均は，
\begin{equation}
\mu_Z = E[Z] = E[X + Y] = E[X] + E[Y] = \mu_X + \mu_Y
\end{equation}
よって，分散は，
\begin{equation}
\begin{split}
V(X + Y) & = V(Z) = E[(Z - \mu_Z)^2] \\
	& = E[\qty{(X + Y) - (\mu_X + \mu_Y)}^2]\\
	& = E[\qty{(X - \mu_X) - (Y - \mu_Y)}^2] \\
	& = E[(X - \mu_X)^2 + 2(X - \mu_X)(Y - \mu_Y) + (Y - \mu_Y)^2] \\
	& = E[(X - \mu_X)] + E[(Y - \mu_Y)^2] + 2E[(X - \mu_X)(Y - \mu_Y)] \\
	& = V(X) + V(Y) + 2Cov(X, Y)
\end{split}
\end{equation}


\subsection*{3.}
2.より，$X$と$Y$が無相関（$Cov(X, Y) = 0$）のとき，
\begin{equation}
V(X + Y) = V(X) + V(Y)
\end{equation}


\end{document}